Suffixes for labeled with lists

Labeled/Lists/OkLib.v
@@ -5,21 +5,21 @@ Require Import LibTactics. (* case_if *)
 
 Open Scope permut_scope.
 
-Fixpoint ok_Gamma (G: Context_L) (Used: list var) : Prop :=
+Fixpoint ok_Gamma_L (G: ctx_L) (Used: list var) : Prop :=
 match G with
 | nil => True
-| (w, (v, A)) :: G' => ~ Mem v Used /\ ok_Gamma G' (v::Used)
+| (w, (v, A)) :: G' => ~ Mem v Used /\ ok_Gamma_L G' (v::Used)
 end.
 
-Fixpoint ok_Omega (L: list var) : Prop :=
+Fixpoint ok_Omega_L (L: list var) : Prop :=
 match L with
 | nil => True
-| l :: L' => ~ Mem l L' /\ ok_Omega L'
+| l :: L' => ~ Mem l L' /\ ok_Omega_L L'
 end.
 
-Lemma ok_Gamma_used_permut:
+Lemma ok_Gamma_L_used_permut:
 forall G U U',
-  U *=* U' -> ok_Gamma G U -> ok_Gamma G U'.
+  U *=* U' -> ok_Gamma_L G U -> ok_Gamma_L G U'.
 induction G; intros.
 destruct U'; econstructor; eauto.
 destruct a; destruct p; simpl in *; destruct H0; split.
@@ -27,20 +27,20 @@ intro n; elim H0; apply Mem_permut with (l:=U'); [ symmetry | ]; auto.
 eapply IHG; eauto.
 Qed.
 
-Lemma ok_Gamma_weakening_used:
+Lemma ok_Gamma_L_weakening_used:
 forall G U u,
-  ok_Gamma G (u::U) ->
-  ok_Gamma G U.
+  ok_Gamma_L G (u::U) ->
+  ok_Gamma_L G U.
 induction G; intros; try constructor.
 destruct a; destruct p; simpl in *; destruct H; split.
 intro; elim H; rewrite Mem_cons_eq; right; auto.
-apply ok_Gamma_used_permut with (U' := (u::v0::U)) in H0;
+apply ok_Gamma_L_used_permut with (U' := (u::v0::U)) in H0;
 [ | permut_simpl]; apply IHG with (u:=u); auto.
 Qed.
 
-Lemma ok_Gamma_permut:
+Lemma ok_Gamma_L_permut:
 forall G1 G2 U,
-  G1 *=* G2 -> ok_Gamma G1 U -> ok_Gamma G2 U.
+  G1 *=* G2 -> ok_Gamma_L G1 U -> ok_Gamma_L G2 U.
 induction G1; intros.
 apply permut_nil_eq in H; subst; auto.
 destruct a; destruct p; simpl in *; destruct H0.
@@ -59,13 +59,13 @@ intro; elim H; rewrite Mem_cons_eq; right; auto.
 apply IHhd with (G1:=hd++tl); try permut_simpl.
 intro n; elim H; rewrite Mem_cons_eq in n; destruct n; rewrite Mem_cons_eq;
 [left; subst; auto | contradiction].
-apply ok_Gamma_used_permut with (U:=v2::v0::U); [permut_simpl | auto].
+apply ok_Gamma_L_used_permut with (U:=v2::v0::U); [permut_simpl | auto].
 intros; auto.
 Qed.
 
-Lemma ok_Omega_permut:
+Lemma ok_Omega_L_permut:
 forall O1 O2,
-  O1 *=* O2 -> ok_Omega O1 -> ok_Omega O2.
+  O1 *=* O2 -> ok_Omega_L O1 -> ok_Omega_L O2.
 induction O1; intros.
 apply permut_nil_eq in H; subst; auto.
 simpl in *; destruct H0.
@@ -92,20 +92,20 @@ intro n. elim H0. apply Mem_permut with (l:=a0::hd++tl).
 symmetry; auto. rewrite Mem_cons_eq; right; auto.
 Qed.
 
-Definition ok_L Omega Gamma := ok_Omega Omega /\ ok_Gamma Gamma nil.
+Definition ok_L Omega Gamma := ok_Omega_L Omega /\ ok_Gamma_L Gamma nil.
 
 Lemma ok_L_permut:
 forall O O' G G', O *=* O' -> G *=* G' -> ok_L O G -> ok_L O' G'.
 intros; destruct H1; split;
-[eapply ok_Omega_permut | eapply ok_Gamma_permut]; eauto.
+[eapply ok_Omega_L_permut | eapply ok_Gamma_L_permut]; eauto.
 Qed.
 
-Lemma ok_Gamma_extend_fresh:
+Lemma ok_Gamma_L_extend_fresh:
 forall G U x w A,
-  ok_Gamma G U ->
+  ok_Gamma_L G U ->
   x \notin used_vars_context_L G ->
   ~ Mem x U ->
-  ok_Gamma ((w, (x, A))::G) U.
+  ok_Gamma_L ((w, (x, A))::G) U.
 induction G; intros; simpl in *; split; auto;
 destruct a; destruct p; destruct H; split.
 rewrite Mem_cons_eq; intro n; destruct n; subst.
@@ -113,7 +113,7 @@ unfold used_vars_context_L in H0; rew_map in *; simpl in *;
 rewrite from_list_cons in H0; rewrite notin_union in H0; destruct H0;
 apply notin_singleton in H0; elim H0; auto.
 contradiction.
-apply ok_Gamma_used_permut with (U:=x::v0::U). permut_simpl.
+apply ok_Gamma_L_used_permut with (U:=x::v0::U). permut_simpl.
 apply IHG; auto.
 unfold used_vars_context_L in *; rew_map in *; simpl in *;
 rewrite from_list_cons in H0; rewrite notin_union in H0; destruct H0; auto.
@@ -129,7 +129,7 @@ forall O G x w A,
   x \notin used_vars_context_L G ->
   ok_L O ((w, (x, A))::G).
 unfold ok_L; intros; destruct H; split; auto.
-apply ok_Gamma_extend_fresh; auto.
+apply ok_Gamma_L_extend_fresh; auto.
 rewrite Mem_nil_eq; tauto.
 Qed.
 
@@ -140,7 +140,7 @@ forall w x A Gamma Omega B,
   False.
 unfold ok_L; intros; simpl in *; destruct H0; destruct H1.
 apply Mem_split in H; destruct H as (hd, (tl, H)); subst.
-apply ok_Gamma_permut with (G2:=(w, (x,A))::hd++tl) in H2.
+apply ok_Gamma_L_permut with (G2:=(w, (x,A))::hd++tl) in H2.
 simpl in H2; destruct H2.
 elim H; apply Mem_here.
 permut_simpl.
@@ -151,20 +151,20 @@ forall O X w x a,
   ok_L O ((w, (x, a)) :: X)  ->
   ok_L O X.
 unfold ok_L; intros; split; destruct H; auto.
-simpl in *; destruct H0; apply ok_Gamma_weakening_used with (u:=x); auto.
+simpl in *; destruct H0; apply ok_Gamma_L_weakening_used with (u:=x); auto.
 Qed.
 
 Lemma ok_L_Mem_contr:
 forall X w x a U,
-  ok_Gamma ((w, (x, a)) :: X) U  ->
+  ok_Gamma_L ((w, (x, a)) :: X) U  ->
   forall w' b, ~ Mem (w', (x, b)) X.
 intros; intro n; simpl in *; destruct H.
 apply Mem_split in n; destruct n as (hd, (tl, n)); subst.
-apply ok_Gamma_permut with (G2:= (w', (x, b))::hd ++ tl) in H0;
+apply ok_Gamma_L_permut with (G2:= (w', (x, b))::hd ++ tl) in H0;
 [|permut_simpl]; simpl in *; destruct H0; elim H0; apply Mem_here.
 Qed.
 
-Fixpoint rename_context_L (w: var) (w': var) (C: Context_L) :=
+Fixpoint rename_context_L (w: var) (w': var) (C: ctx_L) :=
 match C with
 | nil => nil
 | (w0, (x, A)) :: C'  =>
@@ -172,10 +172,10 @@ match C with
     (w1, (x, A)) :: (rename_context_L w w' C')
 end.
 
-Lemma ok_Gamma_rename:
+Lemma ok_Gamma_L_rename:
 forall G U w w',
-  ok_Gamma G U ->
-  ok_Gamma (rename_context_L w w' G) U.
+  ok_Gamma_L G U ->
+  ok_Gamma_L (rename_context_L w w' G) U.
 induction G; intros; simpl in *; auto;
 destruct a; destruct p; simpl in *; destruct H; split; auto.
 Qed.
@@ -185,7 +185,7 @@ forall Omega Gamma w w',
   ok_L Omega Gamma ->
   ok_L Omega (rename_context_L w w' Gamma).
 unfold ok_L; split; destruct H; auto;
-apply ok_Gamma_rename; auto.
+apply ok_Gamma_L_rename; auto.
 Qed.
 
 Lemma Mem_rename_context_L:
